Automaton.thy
@@ -104,6 +104,12 @@ lemma stepstep_step: "spfStep In Out\<cdot>f\<rightleftharpoons>sb = (f ((inv co
 
 section \<open>Lemma about h\<close>
 
+lemma h_dom [simp]: "spfDom\<cdot>(h automat s) = getDom automat"
+  by (metis (no_types, lifting) Abs_cfun_inverse2 h_cont h_def spfStateFix_fix spfstep_dom spfstep_ran)
+
+lemma h_ran [simp]: "spfRan\<cdot>(h automat s) = getRan automat"
+  by (metis spf_ran_2_tsbdom2 spfstep_dom spfstep_ran stepstep_step)
+
 lemma h_unfolding: "(h automat s) = spfStep (getDom automat) (getRan automat)\<cdot>(helper (getTransition automat) s\<cdot>(h automat))"
   by (metis (no_types, lifting) Abs_cfun_inverse2 h_cont h_def spfStateFix_fix spfstep_dom spfstep_ran)
 
@@ -117,10 +123,12 @@ definition autGetNextOutput:: "('s::type, 'm::message) automaton \<Rightarrow> '
 "autGetNextOutput aut s m = snd ((getTransition aut) (s,m))"
 
 (* ToDo: make a bit more readable *)
-lemma h_final: "(h automat s)\<rightleftharpoons>sb = 
+lemma h_final: 
+  assumes "sbDom\<cdot>sb = getDom automat"
+  shows "(h automat s)\<rightleftharpoons>sb = 
   spfConc (autGetNextOutput automat s ((inv convDiscrUp)(sbHdElem\<cdot>sb)))\<cdot>(spfRt\<cdot>(h automat (autGetNextState automat s ((inv convDiscrUp)(sbHdElem\<cdot>sb))))) \<rightleftharpoons>sb"
   unfolding h_step
-  by(simp add: helper_def autGetNextOutput_def autGetNextState_def)
+  by(simp add: helper_def autGetNextOutput_def autGetNextState_def assms spfRt_def)
   
 
 section \<open>Lemma about H\<close>
